\begin{enumerate}
    \item \label{P1}
          Let \(x,y \in \mathbb{R}, \ x < y\) and \(n \in \mathbb{N}\). Define \(\delta  := \frac{y - x}{n}\):
          \begin{align}
              \abs{f(x)  - f(y)} & \leq \sum_{i = 1}^{n}{\abs{f(x + i\delta) - f(x + (i-1)\delta)}} \\
                                 & \leq \sum_{i = 1}^{n}{\abs{x + i\delta - (x + (i-1)\delta)}^2}   \\
                                 & = n \delta^2 = \dfrac{(y -x)^2}{n}                               \\
              \implies           & \abs{f(x) - f(y)} = 0,\qquad \forall x,y \in \mathbb{R}          \\
              \implies           & f(x) \equiv c
          \end{align}
    \item \leavevmode
          \begin{enumerate}
              \item
                    \(f(x)\) is uniformly continuous by letting \(\delta = \left(\frac{\epsilon}{H + 1}\right)^\frac{1}{\alpha}\). Since \(f(x)\) is continuous then for any sequence \(\{x_n\}\) such that \(x_n \to a\), \(\{f(x_n)\}\) is convergent. Let its limit to be \(L_a\). Define \(L_b\) similarly for \(b\). Then by the uniqueness of the limits
                    \begin{equation}
                        g(x) = \begin{cases}
                            f(x) & a < x < b \\
                            L_a  & x = a     \\
                            L_b  & x = b
                        \end{cases}
                    \end{equation}
                    is unique and continuous. WLOG we prove that:
                    \begin{equation}
                        \forall x \in [a,b] \ \abs{g(x) - g(a)} \leq 2H\abs{x - a}^\alpha
                    \end{equation}
                    let \(x_n \to a\) and fix \(\epsilon \leq H\abs{x - a}^\alpha\). Then for some \(n >= N_g\) we have:
                    \begin{equation}
                        \begin{cases}
                            \abs{g(x_n)- g(a)} < \epsilon               \\
                            x_n < x \implies \abs{x_n -a} < \abs{x - a} \\
                        \end{cases}
                    \end{equation}
                    thus:
                    \begin{align}
                        \abs{g(a) - g(x)} & \leq \abs{g(a) - g(x_n)} + \abs{g(x_n) - g(x)}                       \\
                                          & \leq \epsilon + H\abs{x_n - x}^\alpha                                \\
                                          & \leq H\abs{x - a}^\alpha + H\abs{a-x}^\alpha = 2H \abs{x - a}^\alpha
                    \end{align}
              \item
                    it means ur mama gay.
              \item
                    same as \cref{P1}.
          \end{enumerate}
    \item
          \begin{enumerate}
              \item use mean value theorem
              \item increasing (not strict).
          \end{enumerate}
    \item conjugate / l'Hopital
    \item true by MVT.
          \begin{equation}
              \lim_{x \to 0}{\dfrac{f(x) - f(0)}{x}} = \lim_{x \to 0}{f'(c_x)} = L
          \end{equation}
    \item [Old book 6.] because of the endpoint can be the minimum and thus they only need to smaller from the values to one side, not both.
    \item l'Hopital proof
    \item l'Hopital proof
    \item \(f(x) = \sqrt{1 - x^2}\) - it seems to follow MVT
    \item define \(g(x) = f(x) - x\) bound it by a linear function. Prove existence and then use monoticity to prove uniqueness.
    \item no clue
    \item By Taylor's theorem:
          \begin{align}
              \lim_{h \to 0}{\dfrac{f(x+h) - f(x) - f'(x)h - \dfrac{f''(x)}{2} h^2}{h^2}} & = 0
              \\
              \lim_{h \to 0}{\dfrac{f(x-h) - f(x) + f'(x)h - \dfrac{f''(x)}{2} h^2}{h^2}} & = 0
              \\
              \implies \lim_{h \to 0}{\dfrac{f(x+h)  -2 f(x) + f(x-h) - f''(x) h^2}{h^2}} & = 0
          \end{align}
          \(f(x) = x^2\sin{\dfrac{1}{x}}\)
    \item for (i) and (ii) simply use the conditions to bound the following, also use the fact that limit exists ofcourse.
          \begin{align}
               & \abs{\dfrac{1}{\beta_n - \alpha_n}}\abs{f(\beta_n) - f(\alpha_n) - (\beta_n - \alpha_n)f'(0)}                                                                                               \\
               & \leq \abs{\dfrac{1}{\beta_n - \alpha_n}}\abs{f(\beta_n) - f(0) - \beta_n f'(0)} + \abs{\dfrac{1}{\beta_n - \alpha_n}}\abs{ f(\alpha_n) - f(0) - \alpha_n f'(0)}                             \\
               & = \abs{\dfrac{\beta_n}{\beta_n - \alpha_n}}\abs{\dfrac{f(\beta_n) - f(0)}{\beta_n} - f'(0)} + \abs{\dfrac{\alpha_n}{\beta_n - \alpha_n}}\abs{ \dfrac{f(\alpha_n) - f(0)}{\alpha_n} - f'(0)}
          \end{align}
          for (iii) use MVT and by continuity of derivative arrive at the desired result. for (b) do the work, no biggie :))
    \item hint induction
    \item \(f(x) = x^{r+1}\sin{\dfrac{1}{x}} \in \mathcal{C}^r\) but it not \(\mathcal{C}^{r+1}\)
    \item \leavevmode
          \begin{enumerate}
              \item Clearly on the derivative at \(x = 0\) may fail to exist. We claim that \(\frac{d^n}{dx^n}\mathcal{E}(0) = 0\)
              \item yes it is analytic.
              \item the product of two smooth function is smooth. the rest is obvious
          \end{enumerate}
    \item \(L\) is closed then \(U = L^c\) is open in \(\mathbb{R}\). Therefore there are countable disjoint open intervals \(I_n\) such that \(U = \cup I_n\). Let \(I_i = ]a_i,b_i[\). Define:
          \begin{equation}
              \beta_L(x) = \sum_{i = 1}^{\infty}{e^2 \mathcal{E}(x -a_i) \mathcal{E}(b_i - x)}
          \end{equation}
\end{enumerate}
